
\documentclass{article}
\usepackage{amsmath}
\usepackage{ctex}
%%%%%%%%%%%%%%%%%%%%%%%%%%%%%%%%%%%%%%%%%%%%%%%%%%%%%%%%%%%%%%%%%%%%%%%%%%%%%%%%%%%%%%%%%%%%%%%%%%%%%%%%%%%%%%%%%%%%%%%%%%%%%%%%%%%%%%%%%%%%%%%%%%%%%%%%%%%%%%%%%%%%%%%%%%%%%%%%%%%%%%%%%%%%%%%%%%%%%%%%%%%%%%%%%%%%%%%%%%%%%%%%%%%%
%TCIDATA{OutputFilter=LATEX.DLL}
%TCIDATA{Version=5.00.0.2552}
%TCIDATA{<META NAME="SaveForMode" CONTENT="1">}
%TCIDATA{Created=Wednesday, November 11, 2015 17:31:06}
%TCIDATA{LastRevised=Wednesday, November 11, 2015 22:44:17}
%TCIDATA{<META NAME="GraphicsSave" CONTENT="32">}
%TCIDATA{<META NAME="DocumentShell" CONTENT="Standard LaTeX\Blank - Standard LaTeX Article">}
%TCIDATA{CSTFile=40 LaTeX article.cst}

\newtheorem{theorem}{Theorem}
\newtheorem{acknowledgement}[theorem]{Acknowledgement}
\newtheorem{algorithm}[theorem]{Algorithm}
\newtheorem{axiom}[theorem]{Axiom}
\newtheorem{case}[theorem]{Case}
\newtheorem{claim}[theorem]{Claim}
\newtheorem{conclusion}[theorem]{Conclusion}
\newtheorem{condition}[theorem]{Condition}
\newtheorem{conjecture}[theorem]{Conjecture}
\newtheorem{corollary}[theorem]{Corollary}
\newtheorem{criterion}[theorem]{Criterion}
\newtheorem{definition}[theorem]{Definition}
\newtheorem{example}[theorem]{Example}
\newtheorem{exercise}[theorem]{Exercise}
\newtheorem{lemma}[theorem]{Lemma}
\newtheorem{notation}[theorem]{Notation}
\newtheorem{problem}[theorem]{Problem}
\newtheorem{proposition}[theorem]{Proposition}
\newtheorem{remark}[theorem]{Remark}
\newtheorem{solution}[theorem]{Solution}
\newtheorem{summary}[theorem]{Summary}
\newenvironment{proof}[1][Proof]{\noindent\textbf{#1.} }{\ \rule{0.5em}{0.5em}}
\input{macros.tex}

\begin{document}


1.$\left( 1\right) $恒等式为关于$x^{k}$%
的Langrage插值多项式,因而%
成立.

$\left( 2\right) \underset{j=0}{\overset{n}{\sum }}\left( x_{j}-x\right)
^{k}l_{j}\left( x\right) =\underset{j=0}{\overset{n}{\sum }}\underset{t=0}{%
\overset{k}{\sum }}\binom{k}{t}x_{j}^{t}\left( -x\right) ^{k-t}l_{j}\left(
x\right) =\underset{t=0}{\overset{k}{\sum }}\binom{k}{t}\left( -x\right)
^{k-t}\underset{j=0}{\overset{n}{\sum }}x_{j}^{t}l_{j}\left( x\right) $

$\bigskip $由$\left( 1\right) $的结论$\underset{j=0}{%
\overset{n}{\sum }}x_{j}^{t}l_{j}\left( x\right) =x^{t},$因此%
上式可化为

$=\underset{k=0}{\overset{m}{\sum }}\binom{k}{t}\left( -x\right)
^{k-t}x^{t}=\left( x-x\right) ^{k}=0,$for $k\neq 0.$

\bigskip $E\left( \left( \frac{\partial }{\partial \theta }\log f\left(
X|\theta \right) \right) ^{2}\right) =\int \left( \frac{\frac{\partial }{%
\partial \theta }f\left( \vec{x}|\theta \right) }{f\left( \vec{x}|\theta
\right) }\right) ^{2}f\left( \vec{x}|\theta \right) d\vec{x}$=$\int \frac{%
\left( \frac{\partial }{\partial \theta }f\left( \vec{x}|\theta \right)
\right) ^{2}}{f\left( \vec{x}|\theta \right) }d\vec{x}$

$-E\left( \frac{\partial ^{2}}{\partial \theta ^{2}}\log f\left( X|\theta
\right) \right) =-\int \left( \frac{\partial }{\partial \theta }\frac{\frac{%
\partial }{\partial \theta }f\left( \vec{x}|\theta \right) }{f\left( \vec{x}%
|\theta \right) }\right) f\left( \vec{x}|\theta \right) d\vec{x}$

$=-\int \left( \frac{f\left( \vec{x}|\theta \right) \frac{\partial ^{2}}{%
\partial \theta ^{2}}f\left( \vec{x}|\theta \right) -\frac{\partial }{%
\partial \theta }f\left( \vec{x}|\theta \right) ^{2}}{f\left( \vec{x}|\theta
\right) }\right) d\vec{x}=-\int \frac{\partial ^{2}}{\partial \theta ^{2}}%
f\left( \vec{x}|\theta \right) d\vec{x}+\int \frac{\frac{\partial }{\partial
\theta }f\left( \vec{x}|\theta \right) ^{2}}{f\left( \vec{x}|\theta \right) }%
d\vec{x}$

The condition says that $\frac{d}{d\theta }\int \frac{\partial }{\partial
\theta }f\left( \vec{x}|\theta \right) d\vec{x}=\int \frac{\partial ^{2}}{%
\partial \theta ^{2}}f\left( \vec{x}|\theta \right) d\vec{x}$

Then $E\left( \left( \frac{\partial }{\partial \theta }\log f\left( X|\theta
\right) \right) ^{2}\right) =-\frac{d}{d\theta }\int \frac{\partial }{%
\partial \theta }f\left( \vec{x}|\theta \right) d\vec{x}+\int \frac{\frac{%
\partial }{\partial \theta }f\left( \vec{x}|\theta \right) ^{2}}{f\left( 
\vec{x}|\theta \right) }d\vec{x}$

To prove the equality, we must further assume that 

$\int \frac{\partial }{\partial \theta }f\left( \vec{x}|\theta \right) d\vec{%
x}=\frac{\partial }{\partial \theta }$ $\int f\left( \vec{x}|\theta \right) d%
\vec{x}=1.$ The condition expression on the textbook is
not clear, which does not give this assumption, though it is contained in
the proof of C-R Inequality. See, for example, "Theory of Point Estimation",
by Lehmann
and Casella, 1998 by Springer on page 116 Lemma 5.3, which clearly gives out
necessary conditions for this convenient expression of Fisher Information.

%FRAME

\end{document}
